theories/rules/rules_Mov.v
@@ -55,7 +55,7 @@ Section cap_lang_rules.
     iApply wp_wp2.
     iApply wp_opt2_bind.
     iApply wp_opt2_eqn.
-    iMod (state_interp_transient_intro (lm:= ∅) with "[$Hmap $Hσ1]") as "Hσ".
+    iDestruct (state_interp_transient_intro (lm:= ∅) with "[$Hmap $Hσ1]") as "Hσ".
     { by rewrite big_sepM_empty. }
     iApply (wp2_word_of_argument (lrt := lregs) (lw := lw) with "[$Hσ Hφ Hpc_a Hcred]"); first by set_solver.
     iIntros (lw2) "Hσ %Heqlw2 %Heqw2".
